Cleanup after refactoring without modules.

Rewriting.v
@@ -1,187 +1,159 @@
-Require Import Term.
-
-Add LoadPath "../".
-Require Import Cantor.epsilon0.EPSILON0.
-
-(* If a + 1 < b then a < b *)
-Axiom lt_invariant_succ : forall a b, succ a < b -> a < b.
-
-(* If a < b and b < c then a < c *)
-Axiom lt_trans : forall a b c, a < b -> b < c -> a < c.
-
-(* Use T1 as type for ordinal numbers *)
-Definition Ord := T1.
-Variable limit : Ord -> Prop.
-Delimit Scope cantor_scope with ord.
-
-Close Scope cantor_scope.
+Require Export Term.
+Require Import Ordinals.
 
 
-Module Type Trs (S : Signature) (X : Variables).
+Section Rules.
 
-  Module T := Terms S X.
-  Export T.
+Variable F : Signature.
+Variable X : Variables.
 
-  (* Rewriting rule consists of two finite terms *)
-  (* TODO: explore alternative using 'term' with proof of finiteness *)
-  Record rule : Set := {
-    lhs     : finite_term;
-    rhs     : finite_term;
-    rule_wf : not_var lhs /\ incl (vars rhs) (vars lhs)
-  }.
+Notation finite_term := (finite_term F X).
 
-  Definition trs := list rule.
+(* Rewriting rules of finite terms *)
+Record rule : Type := {
+  lhs     : finite_term;
+  rhs     : finite_term;
+  rule_wf : not_var lhs /\ incl (vars rhs) (vars lhs)
+}.
 
-  Parameter rules : trs.
+(* Left hand side is linear *)
+Definition left_linear (r : rule) : Prop :=
+  linear (lhs r).
 
-End Trs.
+(* A Term Rewriting System as a finite list of of rewriting rules *)
+Definition trs := list rule.
+
+(* All rules are left-linear *)
+Fixpoint left_linear_trs (s : trs) : Prop :=
+  match s with
+  | nil   => True
+  | r::rs => left_linear r /\ left_linear_trs rs
+  end.
+
+End Rules.
 
 
-Module Rewriting (S : Signature) (X : Variables) (System : Trs S X).
+Implicit Arguments rule [F X].
+Implicit Arguments lhs [F X].
+Implicit Arguments rhs [F X].
+Implicit Arguments left_linear_trs [F X].
 
-  Import System.
 
-  Parameter all_in : forall r : rule, In r rules.
+Section TRSs.
 
-  (* Left hand side is linear *)
-  Definition left_linear (r : rule) : Prop :=
-    linear (lhs r).
+Variable F : Signature.
+Variable X : Variables.
 
-  (* All rules are left-linear *)
-  Fixpoint left_linear_trs (s : trs) : Prop :=
-    match s with
-    | nil   => True
-    | r::rs => left_linear r /\ left_linear_trs rs
-    end.
+Notation term := (term F X).
 
-  (* Rewriting step *)
-  Inductive step : Set :=
-    | Step : context -> rule -> substitution -> step.
+Variable system : trs F X.
 
-  (* Source term of rewriting step *)
-  Definition source (u : step) : term :=
-    match u with
-    | Step c r s => fill c (substitute s (lhs r))
-    end.
+(* Rewriting step *)
+Inductive step : Type :=
+  | Step : forall r : rule, In r system -> context F X -> substitution F X -> step.
 
-  (* Target term of rewriting step *)
-  Definition target (u : step) : term :=
-    match u with
-    | Step c r s => fill c (substitute s (rhs r))
-    end.
+(* Source term of rewriting step *)
+Definition source (u : step) : term :=
+  match u with
+  | Step r H c s => fill c (substitute s (lhs r))
+  end.
 
-  (* Depth of rule application in rewriting step *)
-  Definition depth (u : step) : nat :=
-    match u with
-    | Step c r s => hole_depth c
-    end.
+(* Target term of rewriting step *)
+Definition target (u : step) : term :=
+  match u with
+  | Step r H c s => fill c (substitute s (rhs r))
+  end.
 
-  (* From now on, the default scope is that of our ordinals *)
-  Local Open Scope cantor_scope.
+(* Depth of rule application in rewriting step *)
+Definition depth (u : step) : nat :=
+  match u with
+  | Step r H c s => hole_depth c
+  end.
 
-  (* Strongly continuous rewriting sequences *)
-  (* TODO: this should rely on a TRS *)
-  Record sequence : Set := {
+Variable term_bis : term -> term -> Prop.
 
-      (* Length of rewriting sequence *)
-      length : Ord;
+(* From now on, the default scope is that of our ordinals *)
+Local Open Scope ordinals_scope.
 
-      (* Projection from ordinals (up to length) to steps *)
-      steps  : forall a : T1, a < length -> step;
+(* Strongly continuous rewriting sequences *)
+Record sequence : Type := {
 
-      (* Successive rewriting steps have equal target/source terms *)
-      continuous_local : 
-        forall a : Ord,
-        forall H : succ a < length,
-        term_eq (target (steps a (lt_invariant_succ a length H)))
-                (source (steps (succ a) H));
+  (* Length of rewriting sequence *)
+  length : Ord;
 
-      (* Approaching any limit ordinal a < length from below,
-         for all n, eventually terms are equal to the limit term up to depth n *)
-      continuous_limit : 
-        forall a : Ord, limit a ->
-        forall H1 : a < length,
-        forall n : nat,
-        exists b, b < a /\
-          forall c, b < c -> forall H2 : c < a,
-          equal_up_to n (source (steps c (lt_trans c a length H2 H1)))
-                        (source (steps a H1));
+  (* Projection from ordinals (up to length) to steps *)
+  steps : forall a : Ord, a < length -> step;
 
-      (* Approaching any limit ordinal < length from below,
-         for all n, eventually the rule applications are below depth n *)
-      continuous_strong :
-        forall a : Ord, limit a ->
-        forall H1 : a < length,
-        forall n : nat,
-        exists b, b < a /\
-          forall c, b < c -> forall H2 : c < a,
-          depth (steps c (lt_trans c a length H2 H1)) > n
-  }.
+  (* Successive rewriting steps have equal target/source terms *)
+  continuous_local : 
+    forall a : Ord,
+    forall H : succ a < length,
+    term_bis (target (steps a (lt_invariant_succ a length H)))
+             (source (steps (succ a) H));
 
-  (* Shorthand for reaching source term at step a in rewriting sequence s *)
-  Definition term_at s (a : Ord) H := source (steps s a H).
-
-  (* If the length of the rewriting sequence is a limit ordinal,
-     for all n, eventually terms are equal up to depth n *)
-  Definition weakly_convergent (s : sequence) : Prop :=
-    limit (length s) ->
+  (* Approaching any limit ordinal a < length from below,
+     for all n, eventually terms are equal to the limit term up to depth n *)
+  continuous_limit : 
+    forall a : Ord, limit a ->
+    forall H1 : a < length,
     forall n : nat,
-    exists b, b < length s /\
-      forall c d, b < c -> b < d ->
-      forall H1 : c < length s, forall H2 : d < length s,
-      equal_up_to n (term_at s c H1)
-                    (term_at s d H2).
+    exists b, b < a /\
+      forall c, b < c -> forall H2 : c < a,
+      equal_up_to n (source (steps c (lt_trans c a length H2 H1)))
+                    (source (steps a H1));
 
-  (* If the length of the rewriting sequence is a limit ordinal,
+  (* Approaching any limit ordinal < length from below,
      for all n, eventually the rule applications are below depth n *)
-  Definition strongly_convergent (s : sequence) : Prop :=
-    limit (length s) ->
+  continuous_strong :
+    forall a : Ord, limit a ->
+    forall H1 : a < length,
     forall n : nat,
-    exists b, b < length s /\
-      forall c, b < c -> forall H : c < length s,
-      depth (steps s c H) > n.
+    exists b, b < a /\
+      forall c, b < c -> forall H2 : c < a,
+      depth (steps c (lt_trans c a length H2 H1)) > n
+}.
 
-  (* Any strongly convergent rewriting sequence is also weakly convergent *)
-  Lemma strong_implies_weak : forall s, strongly_convergent s -> weakly_convergent s.
-  Proof.
-  Admitted.
+(* Shorthand for reaching source term at step a in rewriting sequence s *)
+Definition term_at s (a : Ord) H := source (steps s a H).
 
-  (* Assume we can get a limit term for any weakly convergent rewriting sequence *)
-  (* TODO: This would be a fixpoint using b from weakly_convergent *)
-  Variable limit_term : forall s : sequence, weakly_convergent s -> term.
+(* If the length of the rewriting sequence is a limit ordinal,
+   for all n, eventually terms are equal up to depth n *)
+Definition weakly_convergent (s : sequence) : Prop :=
+  limit (length s) ->
+  forall n : nat,
+  exists b, b < length s /\
+    forall c d, b < c -> b < d ->
+    forall H1 : c < length s, forall H2 : d < length s,
+    equal_up_to n (term_at s c H1)
+                  (term_at s d H2).
 
-  Local Close Scope cantor_scope.
+(* If the length of the rewriting sequence is a limit ordinal,
+   for all n, eventually the rule applications are below depth n *)
+Definition strongly_convergent (s : sequence) : Prop :=
+  limit (length s) ->
+  forall n : nat,
+  exists b, b < length s /\
+    forall c, b < c -> forall H : c < length s,
+    depth (steps s c H) > n.
 
+(* Any strongly convergent rewriting sequence is also weakly convergent *)
+Lemma strong_implies_weak : forall s, strongly_convergent s -> weakly_convergent s.
+Proof.
+Admitted.
 
-  (*
-    Ordinal numbers:
+(* Assume we can get a limit term for any weakly convergent rewriting sequence *)
+(* TODO: This would be a fixpoint using b from weakly_convergent *)
+Variable limit_term : forall s : sequence, weakly_convergent s -> term.
 
-    1) Casteran: http://www.labri.fr/perso/casteran/Cantor
+Lemma compression : left_linear_trs system -> forall s : sequence,
+                    forall SC: strongly_convergent s,
+                    exists s' : sequence,
+                    exists SC' : strongly_convergent s',
+                      length s' < omega /\ (* should be <= *)
+                      term_bis (limit_term s (strong_implies_weak s SC)) (limit_term s' (strong_implies_weak s' SC')).
+Proof.
+Admitted.
 
-       Countable ordinals up to phi0 in Cantor Normal Form:
+Local Close Scope ordinals_scope.
 
-       Inductive T1 : Set :=
-         | zero : T1
-         | cons : T1 -> nat -> T1 -> T1.
-
-       cons a n b represents  omega^a *(S n)  + b
-
-       Type T2 contains countable ordinals up to gamma0 in Veblen Normal Form.
-
-    2) Gimenez:
-
-       Inductive Ord:Set :=
-         | OrdO  : Ord
-         | OrdS  : Ord -> Ord
-         | Limit : (Nat -> Ord) -> Ord.
-
-       In this representation, a limit ordinal (Limit h) is a sort
-       of tree with an infinite width, whose nth child is obtained
-       by applying the function h to n.
-
-  *)
-
-End Rewriting.
-
-
-
+End TRSs.
