Term.v
@@ -2,85 +2,74 @@
   A term datatype with fixed symbol arities.
 *)
 
-
 Require Export List.
 Require Export Bvector.
 
+(* Omit element type and length arguments for vector constructors *)
+Implicit Arguments Vnil [A].
+Implicit Arguments Vcons [A n].
+
+Set Implicit Arguments.
+
+Section Term.
 
 (*
   A Signature contains a decidable set of function symbols and
   an arity function on them.
 *)
-Module Type Signature.
-  Parameter symbol : Set.
-  Axiom eq_symbol_dec : forall f1 f2 : symbol, {f1 = f2} + {f1 <> f2}.
-  Parameter arity : symbol -> nat.
-End Signature.
+Record Signature : Type := mkSignature {
+  symbol :> Set;
+  arity : symbol -> nat;
+  beq_symb : symbol -> symbol -> bool;
+  beq_symb_ok : forall x y, beq_symb x y = true <-> x = y
+}.
 
+Implicit Arguments mkSignature [symbol beq_symb].
+Implicit Arguments arity [s].
+Implicit Arguments beq_symb [s].
+Implicit Arguments beq_symb_ok [s x y].
 
 (*
   A decidable set of variables.
 *)
-Module Type Variables.
-  Parameter variable : Set.
-  Axiom eq_variable_dec : forall v1 v2 : variable, {v1 = v2} + {v1 <> v2}.
-End Variables.
-
-
-(*
-  A concrete implementation of a set of variables using the
-  natural numbers.
-*)
-Module NatVars <: Variables.
-
-  Definition variable := nat.
-
-  Lemma eq_variable_dec : forall v1 v2 : variable, {v1 = v2} + {v1 <> v2}.
-  Proof.
-    intros; decide equality.
-  Qed.
-
-End NatVars.
-
+Record Variables : Type := mkVariables {
+  variable :> Type;
+  beq_var : variable -> variable -> bool;
+  beq_var_ok : forall x y, beq_var x y = true <-> x = y
+}.
 
 (*
   A Term module uses a Signature and a set of variables and
   provides a term datatype over them.
 *)
-Module Terms (S : Signature) (X : Variables).
 
-  (* Use names from signature and variables directly *)
-  Import S.
-  Import X.
+Variable Sig : Signature.
+Variable X : Variables.
 
-  (* Omit element type and length arguments for vector constructors *)
-  Implicit Arguments Vnil [A].
-  Implicit Arguments Vcons [A n].
+(* Infinitary term datatype *)
+CoInductive term : Type :=
+  | Var : X -> term
+  | Fun : forall f : Sig, vector term (arity f) -> term.
 
-  (* Infinitary term datatype *)
-  CoInductive term : Set :=
-    | Var : variable -> term
-    | Fun : forall f : symbol, vector term (arity f) -> term.
+(* Finitary term datatype *)
+Inductive finite_term : Type :=
+  | FVar : X -> finite_term
+  | FFun : forall f : Sig, vector finite_term (arity f) -> finite_term.
 
-  (* Finitary term datatype *)
-  Inductive finite_term : Set :=
-    | FVar : variable -> finite_term
-    | FFun : forall f : symbol, vector finite_term (arity f) -> finite_term.
-
-  (* Finite term is not a variable *)
-  Definition not_var t :=
-    match t with
-    | FVar _   => False
-    | FFun _ _ => True
-    end.
+(* Finite term is not a variable *)
+Definition not_var t :=
+  match t with
+  | FVar _   => False
+  | FFun _ _ => True
+  end.
 
   (* List of variable occurrences in finite term *)
   (* TODO: alternatively use Coq.FSets *)
-  Fixpoint vars (t : finite_term) : list variable :=
+  Fixpoint vars (t : finite_term) : list X :=
     match t with
     | FVar x          => x :: nil
     | FFun f subterms =>
-        let fix vars_subterms n (terms : vector finite_term n) {struct terms} : list variable :=
+        let fix vars_subterms n (terms : vector finite_term n) {struct terms} : list X :=
           match terms with
           | Vnil         => nil
           | Vcons u m us => vars u ++ vars_subterms m us
@@ -121,10 +110,10 @@ Module Terms (S : Signature) (X : Variables).
     end.
 
   (* Type of substitutions of terms for variables *)
-  Definition substitution := variable -> term.
+  Definition substitution := X -> term.
 
   (* The identity substitution *)
-  Definition empty_substitution (x : variable) : term := Var x.
+  Definition empty_substitution (x : X) : term := Var x.
 
   (* Apply a substitution to a finite term *)
   Fixpoint substitute (s : substitution) (t : finite_term) {struct t} : term :=
@@ -140,10 +129,8 @@ Module Terms (S : Signature) (X : Variables).
     end.
 
   (* The empty substitution just builds Var terms from variables *)
-  Lemma empty_substitution_is_id : forall (x : variable), empty_substitution x = Var x.
+  Lemma empty_substitution_is_id : forall (x : X), empty_substitution x = Var x.
   Proof.
-    intros.
-    unfold empty_substitution.
     reflexivity.
   Qed.
 
@@ -164,9 +151,9 @@ Module Terms (S : Signature) (X : Variables).
 
   (* One-hole contexts where a hole can occur at any finite dept *)
   (* TODO: Alternatively define this as term over variables extended with a hole (option variable) *)
-  Inductive context : Set :=
+  Inductive context : Type :=
     | Hole : context
-    | CFun : forall f : symbol, forall i j : nat, i + S j = arity f ->
+    | CFun : forall f : Sig, forall i j : nat, i + S j = arity f ->
                vector term i -> context -> vector term j -> context.
 
   Implicit Arguments CFun [i j].
@@ -182,7 +169,7 @@ Module Terms (S : Signature) (X : Variables).
   Fixpoint vector_append (A : Type) n1 n2 (v1 : vector A n1) (v2 : vector A n2) : vector A (n1 + n2) :=
     match v1 in (vector _ p) return (vector A (p + n2)) with
     | Vnil         => v2
-    | Vcons x n xs => Vcons x (vector_append _ n _ xs v2)
+    | Vcons x n xs => Vcons x (vector_append xs v2)
     end.
 
   Implicit Arguments vector_append [A n1 n2].
@@ -199,7 +186,7 @@ Module Terms (S : Signature) (X : Variables).
     | Vcons x n' v' =>
         match n with
         | 0 => !
-        | S m' => Vcons x (vector_cast A n' v' m' _)
+        | S m' => Vcons x (vector_cast v' _ (m:=m'))
         end
     end.
 
@@ -216,54 +203,40 @@ Module Terms (S : Signature) (X : Variables).
   Fixpoint vector_for_all2 (A B : Type) (R : A -> B -> Prop) n m (v : vector A n) (w : vector B m) {struct v} : Prop :=
     match v, w with
     | Vnil,         Vnil         => True
-    | Vcons a _ v', Vcons b _ w' => R a b /\ vector_for_all2 A B R _ _ v' w'
+    | Vcons a _ v', Vcons b _ w' => R a b /\ vector_for_all2 R v' w'
     | _,            _            => False
     end.
 
-  Implicit Arguments vector_for_all2 [A B n m].
 
   (* Bisimilarity on terms *)
   CoInductive term_eq : term -> term -> Prop :=
-    | VarEq : forall x : variable, term_eq (Var x) (Var x)
-    | FunEq : forall f : symbol, forall subterms1 subterms2 : vector term (arity f),
-                 terms_eq (arity f) subterms1 subterms2 -> term_eq (Fun f subterms1) (Fun f subterms2)
+    | VarEq : forall x : X, term_eq (Var x) (Var x)
+    | FunEq : forall f : Sig, forall subterms1 subterms2 : vector term (arity f),
+                 terms_eq subterms1 subterms2 -> term_eq (Fun f subterms1) (Fun f subterms2)
   with terms_eq : forall n : nat, (vector term n) -> (vector term n) -> Prop :=
-    | Vnil_eq  : terms_eq 0 Vnil Vnil
+    | Vnil_eq  : terms_eq Vnil Vnil
     | Vcons_eq : forall t u : term, forall n : nat, forall v w : (vector term n),
-                   term_eq t u -> terms_eq n v w -> terms_eq (S n) (Vcons t v) (Vcons u w).
+                   term_eq t u -> terms_eq v w -> terms_eq (Vcons t v) (Vcons u w).
 
   Inductive equal_up_to : nat -> term -> term -> Prop :=
       eut_0   : forall t u : term, equal_up_to 0 t u
-    | eut_var : forall n : nat, forall x : variable, equal_up_to n (Var x) (Var x)
-    | eut_fun : forall n : nat, forall f : symbol, forall v w : vector term (arity f), 
-                equal_up_to_vec n (arity f) v w -> equal_up_to (S n) (Fun f v) (Fun f w)
+    | eut_var : forall n : nat, forall x : X, equal_up_to n (Var x) (Var x)
+    | eut_fun : forall n : nat, forall f : Sig, forall v w : vector term (arity f), 
+                equal_up_to_vec n v w -> equal_up_to (S n) (Fun f v) (Fun f w)
   with equal_up_to_vec : nat -> forall m : nat, vector term m -> vector term m -> Prop :=
-      eutv_nil  : forall n, equal_up_to_vec n 0 Vnil Vnil
+      eutv_nil  : forall n, equal_up_to_vec n Vnil Vnil
     | eutv_cons : forall n,  
                   forall t u : term, equal_up_to n t u -> 
-                  forall m : nat, forall v w : vector term m, equal_up_to_vec n m v w -> 
-                  equal_up_to_vec n (S m) (Vcons t v) (Vcons u w).
+                  forall m : nat, forall v w : vector term m, equal_up_to_vec n v w -> 
+                  equal_up_to_vec n (Vcons t v) (Vcons u w).
 
-(*
-Lemma term_eq_to_equal_up_to_n :
-  forall n, 
-  forall t u : term,
-  term_eq t u ->
-  equal_up_to n t u.
-Proof.
+End Term.
 
+Implicit Arguments Var [X Sig].
+Implicit Arguments FVar [X Sig].
 
-
-induction n as [| n IH]; intros t u H.
-constructor.
-destruct H.
-constructor.
-constructor.
-
-
-destruct H; constructor.
-apply IH.
-exact H.
-*)
-
-End Terms.
+(* once more, out of the section *)
+Implicit Arguments mkSignature [symbol beq_symb].
+Implicit Arguments arity [s].
+Implicit Arguments beq_symb [s].
+Implicit Arguments beq_symb_ok [s x y].
